src/program_proof/tulip/program/txn/proph.v
@@ -49,6 +49,21 @@ Section proph.
     iModIntro. by iApply "HΦ".
   Qed.
 
+  Lemma decode_dbmap_map_val mv (wrs : dbmap) :
+    map.map_val mv = Some (Map.untype wrs) →
+    decode_dbmap mv = wrs.
+  Proof.
+    rewrite /decode_dbmap => ->.
+    rewrite /Map.untype.
+    rewrite -map_fmap_compose.
+    apply map_leibniz.
+    intros k.
+    rewrite ?lookup_fmap.
+    destruct (wrs !! k) as [v|] eqn:Heq; rewrite Heq //=.
+    rewrite /to_dbstring/dbval_to_val.
+    destruct v => //=.
+  Qed.
+
   Lemma wp_ResolveCommit
     p (tid : u64) (ts : nat) (wrsP : loc) q (wrs : dbmap) :
     ⊢
@@ -74,12 +89,13 @@ Section proph.
     iMod ("Hclose" with "[Hp]") as "HΦ".
     { iExists (decode_actions pvs').
       rewrite Hts in Hpvs.
-      iSplit.
-      { admit. (* todo: bad definition of decode dbmap *) }
-      iExists _. by iFrame. }
+      rewrite (decode_dbmap_map_val mv wrs) // in Hpvs.
+      iSplit; first by naive_solver.
+      iExists _. by iFrame.
+    }
     iModIntro. iApply "HΦ".
     iFrame "Hmref".
     eauto.
-  Admitted.
+  Qed.
 
 End proph.
